drule.sml
@@ -698,7 +698,7 @@ open SymGraph
 fun depends_t (n,s) t = 
     case view_term t of 
         vVar(n1,s1) => 
-        n = n1 andalso eq_sort(s,s1)
+        n = n1 andalso (* eq_sort(s,s1)*) s = s1
         orelse depends_s (n,s) s1
       | vFun(f,s1,l) => depends_s (n,s) s1 
                        orelse List.exists (depends_t (n,s)) l 
@@ -726,7 +726,7 @@ fun edges_from_fvs nss = List.filter (op<>) (edges_from_fvs0 nss)
 *)
 
 fun edges_from_fvs nss = 
-    List.filter (fn ((n1,s1),(n2,s2)) => n1 <> n2 orelse not $ eq_sort(s1,s2)) (edges_from_fvs0 nss)
+    List.filter (fn ((n1,s1),(n2,s2)) => n1 <> n2 orelse not $ (*eq_sort(s1,s2)*) s1 = s2) (edges_from_fvs0 nss)
 
 
 fun order_of_fvs f = 
@@ -1071,5 +1071,15 @@ fun split_assum th =
           | SOME cj0 => split_assum0 cj0 th
     end
 
+
+(*---------------------------------------------------------------------------*
+ *       A,t1 |- t2                A,t |- F                                  *
+ *     --------------              --------                                  *
+ *     A |- t1 ==> t2               A |- ~t                                  *
+ *---------------------------------------------------------------------------*)
+
+fun neg_disch t th =
+   if eq_form(concl th,FALSE) then negI t th 
+   else disch t th
 
 end
